LeanApi.lean
@@ -16,4 +16,5 @@ import LeanApi.Http.OpenApi
 import LeanApi.Http.Features
 import LeanApi.Http.Multipart
 import LeanApi.Http.Typed
+import LeanApi.Http.Endpoint
 import LeanApi.Props
